draft cont.

Simple_Firewall/Shadowed.thy
@@ -53,7 +53,7 @@ value "rmshadow [SimpleRule \<lparr>iiface = Iface ''+'', oiface = Iface ''+'', 
 
 
 subsection{*A datastructure for sets of packets*}
-  text{*Previous algorithm is not executable because we have no code for @{typ "simple_packet set"}.*}
+text{*Previous algorithm is not executable because we have no code for @{typ "simple_packet set"}.*}
   
   (*assume: no interface wildcards
     then we should be able to store a packet set in the following*)
@@ -63,24 +63,71 @@ subsection{*A datastructure for sets of packets*}
       oiface :: "iface dnf"
       src :: "(ipv4addr \<times> nat) list"
       dst :: "(ipv4addr \<times> nat) list"
-      proto :: "protocol list"
+      proto :: "protocol set"
       sports :: "(16 word \<times> 16 word) list"
       dports :: "(16 word \<times> 16 word) list"
-  
-  fun simple_packet_set_toSet :: "simple_packet_set \<Rightarrow> simple_packet set" where
-    "simple_packet_set_toSet \<lparr>iiface=iif, oiface=oif, src=sip, dst=dip, proto=p, sports=sps, dports=dps \<rparr> = 
-        {p. dnf_to_bool (\<lambda>m. match_iface m (p_iiface p)) iif \<and>
-            dnf_to_bool (\<lambda>m. match_iface m (p_oiface p)) oif \<and> 
-            (\<exists>rng \<in> set sip. simple_match_ip rng (p_src p))}"
-            (*\<dots>*)
-  (*
+    (*
     what can we do with this representation?
                             \<union>    \<inter>                   negate                            is_empty
     iface dnf               @    dnf_and              dnf_not                          ? \<rightarrow> no iface wildcards, should be doable
     cidr list               @    smallest prefix      to bitrange, negate, cidrsplit   []
-    protocol                @    ?              ?                          ?
+    protocol                \<union>    \<inter>                   -                                 = {}
     port-interval list      @    intersect bitrange   bitrange negate                  []
   *)
+
+  fun simple_packet_set_toSet :: "simple_packet_set \<Rightarrow> simple_packet set" where
+    "simple_packet_set_toSet \<lparr>iiface=iifs, oiface=oifs, src=sips, dst=dips, proto=protocols, sports=spss, dports=dpss \<rparr> = 
+        {p. (dnf_to_bool (\<lambda>m. match_iface m (p_iiface p)) iifs) \<and>
+            (dnf_to_bool (\<lambda>m. match_iface m (p_oiface p)) oifs) \<and> 
+            (\<exists>rng \<in> set sips. simple_match_ip rng (p_src p)) \<and>
+            (\<exists>rng \<in> set dips. simple_match_ip rng (p_dst p)) \<and>
+            (\<exists>proto \<in> protocols. match_proto proto (p_proto p)) \<and>
+            (\<exists>rng \<in> set spss. simple_match_port rng (p_sport p)) \<and>
+            (\<exists>rng \<in> set dpss. simple_match_port rng (p_dport p)) }"
+
+  text{*Did we forget anything? no.*}
+  lemma "p \<in> (simple_packet_set_toSet
+                \<lparr>simple_packet_set.iiface=[[Pos iif]], oiface=[[Pos oif]], src=[sip], dst=[dip], proto={protocol}, sports=[sps], dports=[dps] \<rparr>) \<longleftrightarrow>
+         simple_matches \<lparr>simple_match.iiface=iif, oiface=oif, src=sip, dst=dip, proto=protocol, sports=sps, dports=dps \<rparr> p"
+    by(simp add: simple_matches.simps)
+
+  fun optimize :: "simple_packet_set \<Rightarrow> simple_packet_set" where
+    "optimize \<lparr>iiface=iifs, oiface=oifs, src=sips, dst=dips, proto=protocols, sports=spss, dports=dpss \<rparr> = 
+      \<lparr>iiface=iifs, oiface=oifs, (*todo*)
+       src= remdups sips, dst= remdups dips, (*todo: implode ranges?*)
+       proto=protocols, 
+       sports = filter (\<lambda>(s,e). s \<le> e) spss,
+       dports = filter (\<lambda>(s,e). s \<le> e) dpss \<rparr>"
+  lemma "simple_packet_set_toSet (optimize pkts) = simple_packet_set_toSet pkts"
+    proof -
+    { fix pss p
+      have "(\<exists>rng \<in> set (filter (\<lambda>(s,e). s \<le> e) pss). simple_match_port rng p) \<longleftrightarrow> (\<exists>rng \<in> set pss. simple_match_port rng p)"
+        by(induction pss)(auto) }
+    thus ?thesis
+    apply(cases pkts, rename_tac iifs oifs sips dips protocols spss dpss)
+    by simp
+  qed
+
+  fun is_empty :: "simple_packet_set \<Rightarrow> bool" where
+    "is_empty \<lparr>iiface=iifs, oiface=oifs, src=sips, dst=dips, proto=protocols, sports=spss, dports=dpss \<rparr> \<longleftrightarrow>
+        iifs = [] (*todo*) \<or> oifs = [] \<or> (*todo*)
+        sips = [] \<or> dips = [] \<or>
+        protocols = {} \<or>
+        spss = [] \<or> dpss = [] (*TODO*)"
+   lemma "is_empty pkts \<longleftrightarrow> simple_packet_set_toSet pkts = {}"
+     apply(cases pkts, rename_tac iifs oifs sips dips protocols spss dpss)
+     apply(simp)
+     apply(rule iffI)
+      apply(elim disjE, simp_all)
+     oops (* \<longrightarrow> direction holds*)
+
+  fun invert :: "simple_packet_set \<Rightarrow> simple_packet_set" where
+    "invert \<lparr>iiface=iifs, oiface=oifs, src=sips, dst=dips, proto=protocols, sports=spss, dports=dpss \<rparr> = 
+      \<lparr>iiface=dnf_not iifs, oiface=dnf_not oifs,
+             src= sips, dst=  dips, (*todo*)
+             proto=-protocols, 
+             sports = filter (\<lambda>(s,e). s \<le> e) spss,
+             dports = filter (\<lambda>(s,e). s \<le> e) dpss \<rparr>"
   
   (*Idea: replace (\<forall>p\<in>P. \<not> simple_matches m p) by something with uses simple_packet_set*)
   lemma "(\<forall>p\<in>P. \<not> simple_matches m p) \<longleftrightarrow> P \<inter> {p. simple_matches m p} = {}" by auto
@@ -90,7 +137,6 @@ subsection{*A datastructure for sets of packets*}
       Other direction (if it is empty, the it must return true) can be ignored for the soundness (not completeness)
       of the rmshadow algorithm because if the set is not empty, the ruleset is not modified.
       *)
-
 
 
 end
